playability

.lake/build/ir/Games/gameLib/Conditioning.c
@@ -1,6 +1,6 @@
 // Lean compiler output
 // Module: Games.gameLib.Conditioning
-// Imports: Init Games.gameLib.Basic
+// Imports: Init Games.gameLib.Basic Games.gameLib.Termination
 #include <lean/lean.h>
 #if defined(__clang__)
 #pragma clang diagnostic ignored "-Wunused-parameter"
@@ -16,25 +16,34 @@ extern "C" {
 LEAN_EXPORT lean_object* l_zGame__World__wDraw_world__after__fst___rarg(lean_object*, lean_object*, lean_object*);
 lean_object* lean_mk_empty_array_with_capacity(lean_object*);
 LEAN_EXPORT lean_object* l_fst__strat__deconditioned(lean_object*, lean_object*);
+LEAN_EXPORT lean_object* l_zGame__wDraw_state__on__turn___rarg(lean_object*, lean_object*);
+LEAN_EXPORT lean_object* l_zGame__wDraw_history__on__turn___rarg___boxed(lean_object*, lean_object*);
 LEAN_EXPORT lean_object* l___private_Games_gameLib_Conditioning_0__History__on__turn_match__1_splitter(lean_object*);
 LEAN_EXPORT uint8_t l_instDecidableEqListNil___rarg(lean_object*);
 LEAN_EXPORT lean_object* l_Game__World__wDraw_world__after__fst(lean_object*, lean_object*);
 LEAN_EXPORT lean_object* l___private_Games_gameLib_Conditioning_0__History__on__turn_match__1_splitter___rarg___boxed(lean_object*, lean_object*, lean_object*);
+uint8_t l_instDecidablePredNatTurn__fst(lean_object*);
 LEAN_EXPORT lean_object* l_instDecidableEqListNil___rarg___boxed(lean_object*);
 lean_object* lean_array_pop(lean_object*);
 lean_object* lean_array_to_list(lean_object*, lean_object*);
+LEAN_EXPORT lean_object* l_zGame__wDraw_history__on__turn___rarg(lean_object*, lean_object*);
 LEAN_EXPORT lean_object* l_zGame__World__wDraw_world__after__fst(lean_object*, lean_object*);
+LEAN_EXPORT lean_object* l_zGame__wDraw_state__on__turn___rarg___boxed(lean_object*, lean_object*);
 LEAN_EXPORT lean_object* l_fst__strat__deconditioned___rarg___boxed(lean_object*, lean_object*, lean_object*, lean_object*, lean_object*);
 LEAN_EXPORT lean_object* l_snd__strat__deconditioned(lean_object*, lean_object*);
 LEAN_EXPORT lean_object* l_snd__strat__deconditioned___rarg___boxed(lean_object*, lean_object*, lean_object*, lean_object*, lean_object*);
 uint8_t lean_nat_dec_eq(lean_object*, lean_object*);
+lean_object* l_History__on__turn___rarg(lean_object*, lean_object*, lean_object*, lean_object*);
 lean_object* lean_nat_sub(lean_object*, lean_object*);
 LEAN_EXPORT lean_object* l_snd__strat__deconditioned___rarg(lean_object*, lean_object*, lean_object*, lean_object*, lean_object*);
+LEAN_EXPORT lean_object* l_zGame__wDraw_state__on__turn(lean_object*, lean_object*);
 LEAN_EXPORT lean_object* l_Game__World__wDraw_world__after__preHist(lean_object*, lean_object*);
 LEAN_EXPORT lean_object* l_Game__World__wDraw_world__after__preHist___rarg(lean_object*, lean_object*);
 LEAN_EXPORT lean_object* l_instDecidableEqListNil(lean_object*);
 LEAN_EXPORT lean_object* l___private_Games_gameLib_Conditioning_0__History__on__turn_match__1_splitter___rarg(lean_object*, lean_object*, lean_object*);
 lean_object* l_List_redLength___rarg(lean_object*);
+lean_object* lean_nat_add(lean_object*, lean_object*);
+LEAN_EXPORT lean_object* l_zGame__wDraw_history__on__turn(lean_object*, lean_object*);
 LEAN_EXPORT lean_object* l_Game__World__wDraw_world__after__fst___rarg(lean_object*, lean_object*);
 LEAN_EXPORT lean_object* l_fst__strat__deconditioned___rarg(lean_object*, lean_object*, lean_object*, lean_object*, lean_object*);
 lean_object* l_List_toArrayAux___rarg(lean_object*, lean_object*);
@@ -311,8 +320,130 @@ lean_dec(x_1);
 return x_4;
 }
 }
+LEAN_EXPORT lean_object* l_zGame__wDraw_history__on__turn___rarg(lean_object* x_1, lean_object* x_2) {
+_start:
+{
+lean_object* x_3; lean_object* x_4; lean_object* x_5; lean_object* x_6; lean_object* x_7; 
+x_3 = lean_ctor_get(x_1, 0);
+lean_inc(x_3);
+x_4 = lean_ctor_get(x_3, 0);
+lean_inc(x_4);
+lean_dec(x_3);
+x_5 = lean_ctor_get(x_1, 1);
+lean_inc(x_5);
+x_6 = lean_ctor_get(x_1, 2);
+lean_inc(x_6);
+lean_dec(x_1);
+x_7 = l_History__on__turn___rarg(x_4, x_5, x_6, x_2);
+return x_7;
+}
+}
+LEAN_EXPORT lean_object* l_zGame__wDraw_history__on__turn(lean_object* x_1, lean_object* x_2) {
+_start:
+{
+lean_object* x_3; 
+x_3 = lean_alloc_closure((void*)(l_zGame__wDraw_history__on__turn___rarg___boxed), 2, 0);
+return x_3;
+}
+}
+LEAN_EXPORT lean_object* l_zGame__wDraw_history__on__turn___rarg___boxed(lean_object* x_1, lean_object* x_2) {
+_start:
+{
+lean_object* x_3; 
+x_3 = l_zGame__wDraw_history__on__turn___rarg(x_1, x_2);
+lean_dec(x_2);
+return x_3;
+}
+}
+LEAN_EXPORT lean_object* l_zGame__wDraw_state__on__turn___rarg(lean_object* x_1, lean_object* x_2) {
+_start:
+{
+lean_object* x_3; uint8_t x_4; 
+x_3 = lean_unsigned_to_nat(0u);
+x_4 = lean_nat_dec_eq(x_2, x_3);
+if (x_4 == 0)
+{
+lean_object* x_5; lean_object* x_6; lean_object* x_7; lean_object* x_8; uint8_t x_9; 
+x_5 = lean_unsigned_to_nat(1u);
+x_6 = lean_nat_sub(x_2, x_5);
+lean_inc(x_1);
+x_7 = l_zGame__wDraw_history__on__turn___rarg(x_1, x_6);
+x_8 = lean_nat_add(x_6, x_5);
+lean_dec(x_6);
+x_9 = l_instDecidablePredNatTurn__fst(x_8);
+lean_dec(x_8);
+if (x_9 == 0)
+{
+lean_object* x_10; lean_object* x_11; lean_object* x_12; lean_object* x_13; lean_object* x_14; lean_object* x_15; 
+x_10 = lean_ctor_get(x_1, 0);
+lean_inc(x_10);
+x_11 = lean_ctor_get(x_10, 2);
+lean_inc(x_11);
+x_12 = lean_ctor_get(x_10, 0);
+lean_inc(x_12);
+lean_dec(x_10);
+x_13 = lean_ctor_get(x_1, 2);
+lean_inc(x_13);
+lean_dec(x_1);
+lean_inc(x_7);
+lean_inc(x_12);
+x_14 = lean_apply_2(x_13, x_12, x_7);
+x_15 = lean_apply_3(x_11, x_12, x_7, x_14);
+return x_15;
+}
+else
+{
+lean_object* x_16; lean_object* x_17; lean_object* x_18; lean_object* x_19; lean_object* x_20; lean_object* x_21; 
+x_16 = lean_ctor_get(x_1, 0);
+lean_inc(x_16);
+x_17 = lean_ctor_get(x_16, 1);
+lean_inc(x_17);
+x_18 = lean_ctor_get(x_16, 0);
+lean_inc(x_18);
+lean_dec(x_16);
+x_19 = lean_ctor_get(x_1, 1);
+lean_inc(x_19);
+lean_dec(x_1);
+lean_inc(x_7);
+lean_inc(x_18);
+x_20 = lean_apply_2(x_19, x_18, x_7);
+x_21 = lean_apply_3(x_17, x_18, x_7, x_20);
+return x_21;
+}
+}
+else
+{
+lean_object* x_22; lean_object* x_23; 
+x_22 = lean_ctor_get(x_1, 0);
+lean_inc(x_22);
+lean_dec(x_1);
+x_23 = lean_ctor_get(x_22, 0);
+lean_inc(x_23);
+lean_dec(x_22);
+return x_23;
+}
+}
+}
+LEAN_EXPORT lean_object* l_zGame__wDraw_state__on__turn(lean_object* x_1, lean_object* x_2) {
+_start:
+{
+lean_object* x_3; 
+x_3 = lean_alloc_closure((void*)(l_zGame__wDraw_state__on__turn___rarg___boxed), 2, 0);
+return x_3;
+}
+}
+LEAN_EXPORT lean_object* l_zGame__wDraw_state__on__turn___rarg___boxed(lean_object* x_1, lean_object* x_2) {
+_start:
+{
+lean_object* x_3; 
+x_3 = l_zGame__wDraw_state__on__turn___rarg(x_1, x_2);
+lean_dec(x_2);
+return x_3;
+}
+}
 lean_object* initialize_Init(uint8_t builtin, lean_object*);
 lean_object* initialize_Games_gameLib_Basic(uint8_t builtin, lean_object*);
+lean_object* initialize_Games_gameLib_Termination(uint8_t builtin, lean_object*);
 static bool _G_initialized = false;
 LEAN_EXPORT lean_object* initialize_Games_gameLib_Conditioning(uint8_t builtin, lean_object* w) {
 lean_object * res;
@@ -322,6 +453,9 @@ res = initialize_Init(builtin, lean_io_mk_world());
 if (lean_io_result_is_error(res)) return res;
 lean_dec_ref(res);
 res = initialize_Games_gameLib_Basic(builtin, lean_io_mk_world());
+if (lean_io_result_is_error(res)) return res;
+lean_dec_ref(res);
+res = initialize_Games_gameLib_Termination(builtin, lean_io_mk_world());
 if (lean_io_result_is_error(res)) return res;
 lean_dec_ref(res);
 return lean_io_result_mk_ok(lean_box(0));
