Games/gameLib/Termination.lean
@@ -8,7 +8,6 @@ import Games.gameLib.Basic
 
 
 
-
 inductive Game_World_wDraw.Turn_isWLD (g : Game_World_wDraw α β) (f_strat s_strat : Strategy α β) (turn : ℕ) : Prop where
 | wf : Turn_fst turn → g.fst_win_states (g.state_on_turn f_strat s_strat turn) → g.Turn_isWLD f_strat s_strat turn
 | ws : Turn_snd turn → g.snd_win_states (g.state_on_turn f_strat s_strat turn) → g.Turn_isWLD f_strat s_strat turn
